Virtualize actions, states, etc.

ironfleet/src/Dafny/Distributed/Common/Framework/System.s.dfy
@@ -6,29 +6,26 @@ module SystemModule {
     import opened TraceModule
     import opened Native__Io_s
 
-    type ActorState
-    datatype Config = Config(tracked_actors:set<Actor>)
+    type RealActorState
+    datatype RealConfig = RealConfig(tracked_actors:set<RealActor>)
 
-    datatype Connection = Connection(connector:Actor,
+    datatype Connection = Connection(connector:RealActor,
                                      acceptor_ep:EndPoint,
-                                     acceptor:Actor,
+                                     acceptor:RealActor,
                                      closed_by_connector:bool,
                                      closed_by_acceptor:bool,
                                      bytes_pending_for_acceptor:seq<byte>,
                                      bytes_pending_for_connector:seq<byte>)
 
-    datatype SystemState = SystemState(config:Config,
-                                       states:map<Actor, ActorState>,
-                                       time:int,
-                                       connections:map<int, Connection>,
-                                       sent_packets:set<Packet>,
-                                       heap:SharedHeap,
-                                       locks:map<Lock, Actor>)
+    datatype RealSystemState = RealSystemState(config:RealConfig,
+                                               states:map<RealActor, RealActorState>,
+                                               time:int,
+                                               connections:map<int, Connection>,
+                                               sent_packets:set<Packet>,
+                                               heap:SharedHeap,
+                                               locks:map<Lock, RealActor>)
 
-    type SystemBehavior = seq<SystemState>
-
-    predicate HostInit(s:ActorState)
-    predicate HostNextPredicate(s:ActorState, s':ActorState, ios:seq<Event>)
+    type RealSystemBehavior = seq<RealSystemState>
     
     predicate ValidPhysicalIo(event:Event)
     {
@@ -36,17 +33,12 @@ module SystemModule {
         && (event.UdpSendEvent? ==> ValidPhysicalPacket(event.s))
     }
 
-    predicate ValidPhysicalEnvironmentStep(action:Action)
-    {
-        action.ActionVirtual? && action.v.PerformIos? ==> forall io{:trigger io in action.v.raw_ios}{:trigger ValidPhysicalIo(io)} :: io in action.v.raw_ios ==> ValidPhysicalIo(io)
-    }
-
-    predicate ActorStateMatchesInSystemStates(ls:SystemState, ls':SystemState, actor:Actor)
+    predicate ActorStateMatchesInRealSystemStates(ls:RealSystemState, ls':RealSystemState, actor:RealActor)
     {
         if actor in ls.states then (actor in ls'.states && ls'.states[actor] == ls.states[actor]) else actor !in ls'.states
     }
 
-    predicate SystemInit(config:Config, ls:SystemState)
+    predicate RealSystemInit(config:RealConfig, ls:RealSystemState)
     {
            ls.config == config
         && ls.time >= 0
@@ -56,7 +48,7 @@ module SystemModule {
         && ls.locks == map []
     }
 
-    predicate SystemNextUdpReceive(ls:SystemState, ls':SystemState, actor:Actor, p:Packet)
+    predicate RealSystemNextUdpReceive(ls:RealSystemState, ls':RealSystemState, actor:RealActor, p:Packet)
     {
            ls' == ls
         && p in ls.sent_packets
@@ -64,14 +56,14 @@ module SystemModule {
         && p.dst.addr == actor.addr
     }
 
-    predicate SystemNextUdpSend(ls:SystemState, ls':SystemState, actor:Actor, p:Packet)
+    predicate RealSystemNextUdpSend(ls:RealSystemState, ls':RealSystemState, actor:RealActor, p:Packet)
     {
            ls' == ls.(sent_packets := ls.sent_packets + {p})
         && actor.ThreadActor?
         && p.src.addr == actor.addr
     }
 
-    predicate SystemNextTcpConnect(ls:SystemState, ls':SystemState, actor:Actor, conn_id:int, remote_ep:EndPoint)
+    predicate RealSystemNextTcpConnect(ls:RealSystemState, ls':RealSystemState, actor:RealActor, conn_id:int, remote_ep:EndPoint)
     {
            ls' == ls.(connections := ls'.connections)
         && conn_id !in ls.connections
@@ -79,7 +71,7 @@ module SystemModule {
         && ls'.connections == ls.connections[conn_id := Connection(actor, remote_ep, NoActor(), false, false, [], [])]
     }
 
-    predicate SystemNextTcpAccept(ls:SystemState, ls':SystemState, actor:Actor, conn_id:int, remote_ep:EndPoint)
+    predicate RealSystemNextTcpAccept(ls:RealSystemState, ls':RealSystemState, actor:RealActor, conn_id:int, remote_ep:EndPoint)
     {
            conn_id in ls.connections
         && actor.ThreadActor?
@@ -88,7 +80,7 @@ module SystemModule {
         && ls' == ls.(connections := ls.connections[conn_id := ls.connections[conn_id].(acceptor := actor)])
     }
 
-    predicate SystemNextTcpTimeoutReceive(ls:SystemState, ls':SystemState, actor:Actor, conn_id:int, by_connector:bool)
+    predicate RealSystemNextTcpTimeoutReceive(ls:RealSystemState, ls':RealSystemState, actor:RealActor, conn_id:int, by_connector:bool)
     {
            ls' == ls
         && conn_id in ls.connections
@@ -101,7 +93,7 @@ module SystemModule {
                && !conn.closed_by_acceptor
     }
 
-    predicate SystemNextTcpReceive(ls:SystemState, ls':SystemState, actor:Actor, conn_id:int, by_connector:bool, bytes:seq<byte>)
+    predicate RealSystemNextTcpReceive(ls:RealSystemState, ls':RealSystemState, actor:RealActor, conn_id:int, by_connector:bool, bytes:seq<byte>)
     {
            conn_id in ls.connections
         && conn_id in ls'.connections
@@ -118,7 +110,7 @@ module SystemModule {
                   && conn == conn'.(bytes_pending_for_acceptor := bytes + conn'.bytes_pending_for_acceptor)
     }
 
-    predicate SystemNextTcpSend(ls:SystemState, ls':SystemState, actor:Actor, conn_id:int, by_connector:bool, bytes:seq<byte>)
+    predicate RealSystemNextTcpSend(ls:RealSystemState, ls':RealSystemState, actor:RealActor, conn_id:int, by_connector:bool, bytes:seq<byte>)
     {
            conn_id in ls.connections
         && conn_id in ls'.connections
@@ -135,7 +127,7 @@ module SystemModule {
                   && conn' == conn.(bytes_pending_for_connector := conn.bytes_pending_for_connector + bytes)
     }
 
-    predicate SystemNextTcpClose(ls:SystemState, ls':SystemState, actor:Actor, conn_id:int, by_connector:bool)
+    predicate RealSystemNextTcpClose(ls:RealSystemState, ls':RealSystemState, actor:RealActor, conn_id:int, by_connector:bool)
     {
            conn_id in ls.connections
         && conn_id in ls'.connections
@@ -152,27 +144,27 @@ module SystemModule {
                   && conn' == conn.(closed_by_acceptor := true)
     }
 
-    predicate SystemNextReadClock(ls:SystemState, ls':SystemState, actor:Actor, t:int)
+    predicate RealSystemNextReadClock(ls:RealSystemState, ls':RealSystemState, actor:RealActor, t:int)
     {
            ls' == ls
         && !actor.NoActor?
         && t == ls.time
     }
 
-    predicate SystemNextAssumeHeap(ls:SystemState, ls':SystemState, assumption:iset<SharedHeap>)
+    predicate RealSystemNextAssumeHeap(ls:RealSystemState, ls':RealSystemState, assumption:iset<SharedHeap>)
     {
         ls' == ls
         // Note that we DON'T have "assumption in ls.heap" because it's not necessarily justified.
     }
 
-    predicate SystemNextMakeLock(ls:SystemState, ls':SystemState, actor:Actor, lock:Lock)
+    predicate RealSystemNextMakeLock(ls:RealSystemState, ls':RealSystemState, actor:RealActor, lock:Lock)
     {
            ls' == ls.(locks := ls'.locks)
         && lock !in ls.locks
         && ls'.locks == ls.locks[lock := NoActor()]
     }
 
-    predicate SystemNextLock(ls:SystemState, ls':SystemState, actor:Actor, lock:Lock)
+    predicate RealSystemNextLock(ls:RealSystemState, ls':RealSystemState, actor:RealActor, lock:Lock)
     {
            ls' == ls.(locks := ls'.locks)
         && !actor.NoActor?
@@ -181,7 +173,7 @@ module SystemModule {
         && ls'.locks == ls.locks[lock := actor]
     }
 
-    predicate SystemNextUnlock(ls:SystemState, ls':SystemState, actor:Actor, lock:Lock)
+    predicate RealSystemNextUnlock(ls:RealSystemState, ls':RealSystemState, actor:RealActor, lock:Lock)
     {
            ls' == ls.(locks := ls'.locks)
         && !actor.NoActor?
@@ -190,28 +182,28 @@ module SystemModule {
         && ls'.locks == ls.locks[lock := NoActor()]
     }
 
-    predicate SystemNextMakePtr(ls:SystemState, ls':SystemState, actor:Actor, ptr:Ptr<U>, initial_value:U)
+    predicate RealSystemNextMakePtr(ls:RealSystemState, ls':RealSystemState, actor:RealActor, ptr:Ptr<U>, initial_value:U)
     {
            ls' == ls.(heap := ls'.heap)
         && ToU(ptr) !in ls.heap
         && ls'.heap == ls.heap[ToU(ptr) := initial_value]
     }
 
-    predicate SystemNextReadPtr(ls:SystemState, ls':SystemState, actor:Actor, ptr:Ptr<U>, read_value:U)
+    predicate RealSystemNextReadPtr(ls:RealSystemState, ls':RealSystemState, actor:RealActor, ptr:Ptr<U>, read_value:U)
     {
            ls' == ls
         && ToU(ptr) in ls.heap
         && ls.heap[ToU(ptr)] == read_value
     }
 
-    predicate SystemNextWritePtr(ls:SystemState, ls':SystemState, actor:Actor, ptr:Ptr<U>, write_value:U)
+    predicate RealSystemNextWritePtr(ls:RealSystemState, ls':RealSystemState, actor:RealActor, ptr:Ptr<U>, write_value:U)
     {
            ls' == ls.(heap := ls'.heap)
         && ToU(ptr) in ls.heap
         && ls'.heap == ls.heap[ToU(ptr) := write_value]
     }
 
-    predicate SystemNextMakeArray(ls:SystemState, ls':SystemState, actor:Actor, arr:Array<U>, arr_len:int, initial_value:U)
+    predicate RealSystemNextMakeArray(ls:RealSystemState, ls':RealSystemState, actor:RealActor, arr:Array<U>, arr_len:int, initial_value:U)
     {
            ls' == ls.(heap := ls'.heap)
         && ToU(arr) !in ls.heap
@@ -220,7 +212,7 @@ module SystemModule {
                          && (forall i :: 0 <= i < arr_len ==> s[i] == initial_value))
     }
 
-    predicate SystemNextReadArray(ls:SystemState, ls':SystemState, actor:Actor, arr:Array<U>, index:int, read_value:U)
+    predicate RealSystemNextReadArray(ls:RealSystemState, ls':RealSystemState, actor:RealActor, arr:Array<U>, index:int, read_value:U)
     {
            ls' == ls
         && ToU(arr) in ls.heap
@@ -229,7 +221,7 @@ module SystemModule {
                          && s[index] == read_value)
     }
 
-    predicate SystemNextWriteArray(ls:SystemState, ls':SystemState, actor:Actor, arr:Array<U>, index:int, write_value:U)
+    predicate RealSystemNextWriteArray(ls:RealSystemState, ls':RealSystemState, actor:RealActor, arr:Array<U>, index:int, write_value:U)
     {
            ls' == ls.(heap := ls'.heap)
         && ToU(arr) in ls.heap
@@ -238,143 +230,101 @@ module SystemModule {
                          && ls'.heap == ls.heap[ToU(arr) := ToU(s[index := write_value])])
     }
 
-    predicate SystemNextUpdateLocalState(ls:SystemState, ls':SystemState, actor:Actor)
+    predicate RealSystemNextUpdateLocalState(ls:RealSystemState, ls':RealSystemState, actor:RealActor)
     {
            (forall other_actor {:trigger ls.states[other_actor]}{:trigger other_actor in ls.states}{:trigger other_actor in ls'.states} ::
-                           other_actor != actor ==> ActorStateMatchesInSystemStates(ls, ls', other_actor))
+                           other_actor != actor ==> ActorStateMatchesInRealSystemStates(ls, ls', other_actor))
         && ls' == ls.(states := ls'.states)
     }
 
-    predicate SystemNextStutter(ls:SystemState, ls':SystemState)
+    predicate RealSystemNextStutter(ls:RealSystemState, ls':RealSystemState)
     {
         ls' == ls
     }
 
-    predicate SystemNextDeliverPacket(ls:SystemState, ls':SystemState, actor:Actor, p:Packet)
+    predicate RealSystemNextDeliverPacket(ls:RealSystemState, ls':RealSystemState, actor:RealActor, p:Packet)
     {
            p in ls.sent_packets
         && ls' == ls
         && actor.NoActor?
     }
 
-    predicate SystemNextAdvanceTime(ls:SystemState, ls':SystemState, actor:Actor, t:int)
+    predicate RealSystemNextAdvanceTime(ls:RealSystemState, ls':RealSystemState, actor:RealActor, t:int)
     {
            t > ls.time
         && ls' == ls.(time := t)
         && actor.NoActor?
     }
 
-    predicate SystemNextPerformIos(
-        ls:SystemState,
-        ls':SystemState,
-        actor:Actor,
-        ios:seq<Event>
-        )
-    {
-           ls' == ls.(sent_packets := ls'.sent_packets)
-        && (forall p :: p in ls.sent_packets ==> p in ls'.sent_packets)
-        && (forall p :: p in ls'.sent_packets ==> p in ls.sent_packets || UdpSendEvent(p) in ios)
-		&& actor.ThreadActor?
-        && (forall io :: io in ios && io.UdpReceiveEvent? ==> io.r in ls.sent_packets && io.r.dst.addr == actor.addr)
-        && (forall io :: io in ios && io.UdpSendEvent? ==> io.s in ls'.sent_packets && io.s.src.addr == actor.addr)
-    }
-
-    predicate SystemNextHostNext(
-        ls:SystemState,
-        ls':SystemState,
-        actor:Actor,
-        ios:seq<Event>
-        )
-    {
-           ls' == ls.(sent_packets := ls'.sent_packets, states := ls'.states)
-        && actor in ls.states
-        && actor in ls'.states
-        && ls'.states == ls.states[actor := ls'.states[actor]]
-        && HostNextPredicate(ls.states[actor], ls'.states[actor], ios)
-        && (forall p :: p in ls.sent_packets ==> p in ls'.sent_packets)
-        && (forall p :: p in ls'.sent_packets ==> p in ls.sent_packets || UdpSendEvent(p) in ios)
-		&& actor.ThreadActor?
-        && (forall io :: io in ios && io.UdpReceiveEvent? ==> io.r in ls.sent_packets && io.r.dst.addr == actor.addr)
-        && (forall io :: io in ios && io.UdpSendEvent? ==> io.s in ls'.sent_packets && io.s.src.addr == actor.addr)
-    }
-
-    predicate SystemNextVirtualAction(ls:SystemState, ls':SystemState, actor:Actor, action:VirtualAction)
-    {
-        match action
-            case PerformIos(ios) => SystemNextPerformIos(ls, ls', actor, ios)
-            case HostNext(ios) => SystemNextHostNext(ls, ls', actor, ios)
-    }
-
-    predicate SystemNextUntrackedEvent(ls:SystemState, ls':SystemState, actor:Actor, event:UntrackedEvent)
+    predicate RealSystemNextUntrackedEvent(ls:RealSystemState, ls':RealSystemState, actor:RealActor, event:UntrackedEvent)
     {
         match event
-            case UpdateLocalState => SystemNextUpdateLocalState(ls, ls', actor)
-            case DeliverPacket(p) => SystemNextDeliverPacket(ls, ls', actor, p)
-            case AdvanceTime(t) => SystemNextAdvanceTime(ls, ls', actor, t)
+            case UpdateLocalState => RealSystemNextUpdateLocalState(ls, ls', actor)
+            case DeliverPacket(p) => RealSystemNextDeliverPacket(ls, ls', actor, p)
+            case AdvanceTime(t) => RealSystemNextAdvanceTime(ls, ls', actor, t)
     }
 
-    predicate SystemNextTrackedEvent(ls:SystemState, ls':SystemState, actor:Actor, event:Event)
+    predicate RealSystemNextTrackedEvent(ls:RealSystemState, ls':RealSystemState, actor:RealActor, event:Event)
     {
         match event
-            case MakeLockEvent(lock) => SystemNextMakeLock(ls, ls', actor, lock)
-            case LockEvent(lock) => SystemNextLock(ls, ls', actor, lock)
-            case UnlockEvent(lock) => SystemNextUnlock(ls, ls', actor, lock)
-            case AssumeHeapEvent(assumption) => SystemNextAssumeHeap(ls, ls', assumption)
-            case MakePtrEvent(ptr, v) => SystemNextMakePtr(ls, ls', actor, ptr, v)
-            case ReadPtrEvent(ptr, v) => SystemNextReadPtr(ls, ls', actor, ptr, v)
-            case WritePtrEvent(ptr, v) => SystemNextWritePtr(ls, ls', actor, ptr, v)
-            case MakeArrayEvent(arr, len, v) => SystemNextMakeArray(ls, ls', actor, arr, len, v)
-            case ReadArrayEvent(arr, index, v) => SystemNextReadArray(ls, ls', actor, arr, index, v)
-            case WriteArrayEvent(arr, index, v) => SystemNextWriteArray(ls, ls', actor, arr, index, v)
-            case ReadClockEvent(t) => SystemNextReadClock(ls, ls', actor, t)
-            case UdpTimeoutReceiveEvent() => SystemNextStutter(ls, ls')
-            case UdpReceiveEvent(p) => SystemNextUdpReceive(ls, ls', actor, p)
-            case UdpSendEvent(p) => SystemNextUdpSend(ls, ls', actor, p)
-            case TcpConnectEvent(id, ep) => SystemNextTcpConnect(ls, ls', actor, id, ep)
-            case TcpAcceptEvent(id, ep) => SystemNextTcpAccept(ls, ls', actor, id, ep)
-            case TcpTimeoutReceiveEvent(id, by_connector) => SystemNextTcpTimeoutReceive(ls, ls', actor, id, by_connector)
-            case TcpReceiveEvent(id, by_connector, r) => SystemNextTcpReceive(ls, ls', actor, id, by_connector, r)
-            case TcpSendEvent(id, by_connector, s) => SystemNextTcpSend(ls, ls', actor, id, by_connector, s)
-            case TcpCloseEvent(id, by_connector) => SystemNextTcpClose(ls, ls', actor, id, by_connector)
-            case FIopOpenEvent(f) => SystemNextStutter(ls, ls')                 // TODO - fill in
-            case FIopReadEvent(f, bytes) => SystemNextStutter(ls, ls')          // TODO - fill in
-            case FIopCloseEvent(f) => SystemNextStutter(ls, ls')                // TODO - fill in
+            case MakeLockEvent(lock) => RealSystemNextMakeLock(ls, ls', actor, lock)
+            case LockEvent(lock) => RealSystemNextLock(ls, ls', actor, lock)
+            case UnlockEvent(lock) => RealSystemNextUnlock(ls, ls', actor, lock)
+            case AssumeHeapEvent(assumption) => RealSystemNextAssumeHeap(ls, ls', assumption)
+            case MakePtrEvent(ptr, v) => RealSystemNextMakePtr(ls, ls', actor, ptr, v)
+            case ReadPtrEvent(ptr, v) => RealSystemNextReadPtr(ls, ls', actor, ptr, v)
+            case WritePtrEvent(ptr, v) => RealSystemNextWritePtr(ls, ls', actor, ptr, v)
+            case MakeArrayEvent(arr, len, v) => RealSystemNextMakeArray(ls, ls', actor, arr, len, v)
+            case ReadArrayEvent(arr, index, v) => RealSystemNextReadArray(ls, ls', actor, arr, index, v)
+            case WriteArrayEvent(arr, index, v) => RealSystemNextWriteArray(ls, ls', actor, arr, index, v)
+            case ReadClockEvent(t) => RealSystemNextReadClock(ls, ls', actor, t)
+            case UdpTimeoutReceiveEvent() => RealSystemNextStutter(ls, ls')
+            case UdpReceiveEvent(p) => RealSystemNextUdpReceive(ls, ls', actor, p)
+            case UdpSendEvent(p) => RealSystemNextUdpSend(ls, ls', actor, p)
+            case TcpConnectEvent(id, ep) => RealSystemNextTcpConnect(ls, ls', actor, id, ep)
+            case TcpAcceptEvent(id, ep) => RealSystemNextTcpAccept(ls, ls', actor, id, ep)
+            case TcpTimeoutReceiveEvent(id, by_connector) => RealSystemNextTcpTimeoutReceive(ls, ls', actor, id, by_connector)
+            case TcpReceiveEvent(id, by_connector, r) => RealSystemNextTcpReceive(ls, ls', actor, id, by_connector, r)
+            case TcpSendEvent(id, by_connector, s) => RealSystemNextTcpSend(ls, ls', actor, id, by_connector, s)
+            case TcpCloseEvent(id, by_connector) => RealSystemNextTcpClose(ls, ls', actor, id, by_connector)
+            case FIopOpenEvent(f) => RealSystemNextStutter(ls, ls')                 // TODO - fill in
+            case FIopReadEvent(f, bytes) => RealSystemNextStutter(ls, ls')          // TODO - fill in
+            case FIopCloseEvent(f) => RealSystemNextStutter(ls, ls')                // TODO - fill in
     }
 
-    predicate SystemNextAction(ls:SystemState, ls':SystemState, actor:Actor, action:Action)
+    predicate RealSystemNextAction(ls:RealSystemState, ls':RealSystemState, actor:RealActor, action:RealAction)
     {
         match action
-            case ActionEvent(e) => SystemNextTrackedEvent(ls, ls', actor, e)
-            case ActionUntracked(u) => SystemNextUntrackedEvent(ls, ls', actor, u)
-            case ActionVirtual(v) => SystemNextVirtualAction(ls, ls', actor, v)
+            case RealActionEvent(e) => RealSystemNextTrackedEvent(ls, ls', actor, e)
+            case RealActionUntracked(u) => RealSystemNextUntrackedEvent(ls, ls', actor, u)
     }
 
-    predicate SystemNextEntry(ls:SystemState, ls':SystemState, entry:Entry)
+    predicate RealSystemNextEntry(ls:RealSystemState, ls':RealSystemState, entry:RealEntry)
     {
-        SystemNextAction(ls, ls', entry.actor, entry.action)
+        RealSystemNextAction(ls, ls', entry.actor, entry.action)
     }
 
-    predicate SystemNext(ls:SystemState, ls':SystemState)
+    predicate RealSystemNext(ls:RealSystemState, ls':RealSystemState)
     {
-        exists entry :: SystemNextEntry(ls, ls', entry)
+        exists entry :: RealSystemNextEntry(ls, ls', entry)
     }
 
-    predicate IsValidSystemBehavior(config:Config, lb:SystemBehavior)
+    predicate IsValidRealSystemBehavior(config:RealConfig, lb:RealSystemBehavior)
     {
            |lb| > 0
-        && SystemInit(config, lb[0])
-        && (forall i {:trigger SystemNext(lb[i], lb[i+1])} :: 0 <= i < |lb| - 1 ==> SystemNext(lb[i], lb[i+1]))
+        && RealSystemInit(config, lb[0])
+        && (forall i {:trigger RealSystemNext(lb[i], lb[i+1])} :: 0 <= i < |lb| - 1 ==> RealSystemNext(lb[i], lb[i+1]))
     }
 
-    predicate IsValidSystemTraceAndBehaviorSlice(trace:Trace, lb:SystemBehavior)
+    predicate IsValidRealSystemTraceAndBehaviorSlice(trace:RealTrace, lb:RealSystemBehavior)
     {
            |lb| == |trace| + 1
-        && forall i {:trigger SystemNextEntry(lb[i], lb[i+1], trace[i])} :: 0 <= i < |trace| ==> SystemNextEntry(lb[i], lb[i+1], trace[i])
+        && forall i {:trigger RealSystemNextEntry(lb[i], lb[i+1], trace[i])} :: 0 <= i < |trace| ==> RealSystemNextEntry(lb[i], lb[i+1], trace[i])
     }
 
-    predicate IsValidSystemTraceAndBehavior(config:Config, trace:Trace, lb:SystemBehavior)
+    predicate IsValidRealSystemTraceAndBehavior(config:RealConfig, trace:RealTrace, lb:RealSystemBehavior)
     {
-           IsValidSystemTraceAndBehaviorSlice(trace, lb)
-        && SystemInit(config, lb[0])
+           IsValidRealSystemTraceAndBehaviorSlice(trace, lb)
+        && RealSystemInit(config, lb[0])
     }
 }
