ironfleet/src/Dafny/Distributed/Common/Framework/Trace.s.dfy
@@ -8,34 +8,22 @@ module TraceModule {
     // Some possibilities for the actors and actions in a trace
     /////////////////////////////////////////////////////////////////////
 
-    datatype Actor = NoActor() | ThreadActor(addr:IPAddress, pid:int, tid:int) // pid is assumed unique across machines
+    datatype RealActor = NoActor() | ThreadActor(addr:IPAddress, pid:int, tid:int) // pid is assumed unique across machines
 
     datatype UntrackedEvent = UpdateLocalState()
                             | DeliverPacket(p:Packet)
                             | AdvanceTime(new_time:int)
 
-    datatype VirtualAction = PerformIos(raw_ios:seq<Event>)
-                           | HostNext(host_ios:seq<Event>)    // Like PerformIos, but also changes the host's state
-
-    datatype Action = ActionEvent(e:Event)
-                    | ActionUntracked(u:UntrackedEvent)
-                    | ActionVirtual(v:VirtualAction)
-
-    predicate IsTrackedAction(a:Action)
-    {
-        a.ActionEvent?
-    }
-
-    predicate IsRealAction(a:Action)
-    {
-        IsTrackedAction(a) || a.ActionUntracked?
-    }
+    datatype RealAction = RealActionEvent(e:Event)
+                        | RealActionUntracked(u:UntrackedEvent)
 
     /////////////////////////////////////////////////
     // Traces and the entries they're composed of
     /////////////////////////////////////////////////
 
-    datatype Entry = Entry(actor:Actor, action:Action)
+    datatype Entry<Actor, Action> = Entry(actor:Actor, action:Action)
+    type Trace<Actor, Action> = seq<Entry<Actor, Action>>
 
-    type Trace = seq<Entry>
+    type RealEntry = Entry<RealActor, RealAction>
+    type RealTrace = Trace<RealActor, RealAction>
 }
