ironfleet/src/Dafny/Distributed/Concur/EventHandler.i.dfy
@@ -1,15 +1,91 @@
-include "System.i.dfy"
-include "ReductionBasic.i.dfy"
-include "ReductionPlan.i.dfy"
+include "../Common/Framework/System.s.dfy"
+//include "ReductionBasic.i.dfy"
+//include "ReductionPlan.i.dfy"
 
 module EventHandlerModule {
     import opened SystemModule
-    import opened ReductionBasicModule
-    import opened ReductionPlanModule
+//    import opened ReductionBasicModule
+//    import opened ReductionPlanModule
 
-    predicate IoPerformableByItsActor(entry:Entry)
+    datatype VirtualAction = VirtualActionUntrackedEvent(u:UntrackedEvent)
+                           | PerformIos(raw_ios:seq<Event>)
+                           | HostNext(host_ios:seq<Event>)
+
+    type VirtualActorState
+    datatype VirtualSystemState = VirtualSystemState(config:RealConfig,
+                                                     states:map<RealActor, VirtualActorState>,
+                                                     time:int,
+                                                     connections:map<int, Connection>,
+                                                     sent_packets:set<Packet>,
+                                                     heap:SharedHeap,
+                                                     locks:map<Lock, RealActor>)
+
+    predicate HostInit(s:VirtualActorState)
+    predicate HostNextPredicate(s:VirtualActorState, s':VirtualActorState, ios:seq<Event>)
+
+    predicate ValidPhysicalEnvironmentStep(action:VirtualAction)
     {
-        (entry.action.Send? && entry.actor.HostActor? ==> entry.action.s.src == entry.actor.ep)
+        action.PerformIos? ==> forall io{:trigger io in action.raw_ios}{:trigger ValidPhysicalIo(io)} :: io in action.raw_ios ==> ValidPhysicalIo(io)
+    }
+
+    function VirtualSystemStateToRealSystemState(v:VirtualSystemState) : RealSystemState
+    {
+        RealSystemState(v.config, map [], v.time, v.connections, v.sent_packets, v.heap, v.locks)
+    }
+
+    predicate VirtualSystemNextUntrackedEvent(ls:VirtualSystemState, ls':VirtualSystemState, actor:RealActor, event:UntrackedEvent)
+    {
+        var vs := VirtualSystemStateToRealSystemState(ls);
+        var vs' := VirtualSystemStateToRealSystemState(ls');
+        RealSystemNextUntrackedEvent(vs, vs', actor, event)
+    }
+
+    predicate VirtualSystemNextPerformIos(
+        ls:VirtualSystemState,
+        ls':VirtualSystemState,
+        actor:RealActor,
+        ios:seq<Event>
+        )
+    {
+           ls' == ls.(sent_packets := ls'.sent_packets)
+        && (forall p :: p in ls.sent_packets ==> p in ls'.sent_packets)
+        && (forall p :: p in ls'.sent_packets ==> p in ls.sent_packets || UdpSendEvent(p) in ios)
+		&& actor.ThreadActor?
+        && (forall io :: io in ios && io.UdpReceiveEvent? ==> io.r in ls.sent_packets && io.r.dst.addr == actor.addr)
+        && (forall io :: io in ios && io.UdpSendEvent? ==> io.s in ls'.sent_packets && io.s.src.addr == actor.addr)
+    }
+
+    predicate VirtualSystemNextHostNext(
+        ls:VirtualSystemState,
+        ls':VirtualSystemState,
+        actor:RealActor,
+        ios:seq<Event>
+        )
+    {
+           ls' == ls.(sent_packets := ls'.sent_packets, states := ls'.states)
+        && actor in ls.states
+        && actor in ls'.states
+        && ls'.states == ls.states[actor := ls'.states[actor]]
+        && HostNextPredicate(ls.states[actor], ls'.states[actor], ios)
+        && (forall p :: p in ls.sent_packets ==> p in ls'.sent_packets)
+        && (forall p :: p in ls'.sent_packets ==> p in ls.sent_packets || UdpSendEvent(p) in ios)
+		&& actor.ThreadActor?
+        && (forall io :: io in ios && io.UdpReceiveEvent? ==> io.r in ls.sent_packets && io.r.dst.addr == actor.addr)
+        && (forall io :: io in ios && io.UdpSendEvent? ==> io.s in ls'.sent_packets && io.s.src.addr == actor.addr)
+    }
+
+    predicate VirtualSystemNextVirtualAction(ls:VirtualSystemState, ls':VirtualSystemState, actor:RealActor, action:VirtualAction)
+    {
+        match action
+            case VirtualActionUntrackedEvent(u) => VirtualSystemNextUntrackedEvent(ls, ls', actor, u)
+            case PerformIos(ios) => VirtualSystemNextPerformIos(ls, ls', actor, ios)
+            case HostNext(ios) => VirtualSystemNextHostNext(ls, ls', actor, ios)
+    }
+
+/*
+    predicate IoPerformableByItsActor(entry:RealEntry)
+    {
+        (entry.action.UdpSendEvent? && entry.actor.HostActor? ==> entry.action.s.src == entry.actor.ep)
     }
     
     predicate AllIosPerformableByTheirActors(entries:seq<Entry>)
@@ -64,14 +140,14 @@ module EventHandlerModule {
         pivot_index:int
         )
         requires |lb| == |entries| + 1;
-        requires forall i :: 0 <= i < |entries| ==> SystemNextEntry(lb[i], lb[i+1], entries[i]);
+        requires forall i :: 0 <= i < |entries| ==> VirtualSystemNextEntry(lb[i], lb[i+1], entries[i]);
         requires forall i :: 0 <= i < |entries| ==> entries[i].actor == actor;
         requires forall i :: 0 <= i < |entries| ==> IsTrackedAction(entries[i].action);
         requires entry == CombineIoEntriesIntoEntry(actor, entries);
         requires 0 <= pivot_index <= |entries|;
         requires forall i :: 0 <= i < pivot_index ==> EntryIsRightMover(entries[i]);
         requires forall i :: pivot_index < i < |entries| ==> EntryIsLeftMover(entries[i]);
-        ensures  SystemNextEntry(lb[0], lb[|entries|], entry);
+        ensures  VirtualSystemNextEntry(lb[0], lb[|entries|], entry);
     {
         if |entries| == 0 {
             return;
@@ -110,9 +186,9 @@ module EventHandlerModule {
         requires TreeRootPivotValid(tree);
         requires TreeOnlyForActor(tree, actor);
         requires |lb| == |tree.children| + 1;
-        requires forall i :: 0 <= i < |tree.children| ==> SystemNextEntry(lb[i], lb[i+1], tree.children[i].entry);
+        requires forall i :: 0 <= i < |tree.children| ==> VirtualSystemNextEntry(lb[i], lb[i+1], tree.children[i].entry);
         requires tree.reduced_entry == CombineIoEntriesIntoEntry(actor, GetRootEntries(tree.children));
-        ensures  SystemNextEntry(lb[0], last(lb), tree.reduced_entry);
+        ensures  VirtualSystemNextEntry(lb[0], last(lb), tree.reduced_entry);
     {
         var entries := GetRootEntries(tree.children);
         var entry := tree.reduced_entry;
@@ -121,7 +197,7 @@ module EventHandlerModule {
         lemma_IfAllChildrenAreLeavesThenGetLeafEntriesAreChildren(tree);
 
         forall i | 0 <= i < |entries|
-            ensures SystemNextEntry(lb[i], lb[i+1], entries[i]);
+            ensures VirtualSystemNextEntry(lb[i], lb[i+1], entries[i]);
             ensures entries[i].actor == actor;
             ensures IsTrackedAction(entries[i].action);
         {
@@ -152,7 +228,7 @@ module EventHandlerModule {
             && 0 <= tree.pivot_index < left_mover_pos < |tree.children|
             && (forall entry :: entry in other_actor_entries ==> entry.actor != tree.reduced_entry.actor)
             && IsValidSystemTraceAndBehaviorSlice(GetRootEntries(tree.children[..left_mover_pos]) + other_actor_entries, lb)
-            ensures exists ls' :: SystemNextEntry(last(lb), ls', GetRootEntry(tree.children[left_mover_pos]));
+            ensures exists ls' :: VirtualSystemNextEntry(last(lb), ls', GetRootEntry(tree.children[left_mover_pos]));
         {
             var entry := GetRootEntry(tree.children[left_mover_pos]);
             assert EntryIsLeftMover(entry);
@@ -162,7 +238,7 @@ module EventHandlerModule {
 
             assert TreeOnlyForActor(tree.children[left_mover_pos], actor);
             assert IoPerformableByItsActor(entry);
-            assert SystemNextEntry(ls, ls', entry);
+            assert VirtualSystemNextEntry(ls, ls', entry);
         }
     }
 
@@ -187,14 +263,14 @@ module EventHandlerModule {
         var entries := GetRootEntries(tree.children);
         lemma_IfAllChildrenAreLeavesThenGetLeafEntriesAreChildren(tree);
 
-        forall lb:seq<SystemState> {:trigger SystemNextEntry(lb[0], lb[|entries|], entry)}|
+        forall lb:seq<SystemState> {:trigger VirtualSystemNextEntry(lb[0], lb[|entries|], entry)}|
                 |lb| == |entries|+1
-             && (forall i {:trigger SystemNextEntry(lb[i], lb[i+1], entries[i])} ::
-                 0 <= i < |entries| ==> SystemNextEntry(lb[i], lb[i+1], entries[i]))
-            ensures SystemNextEntry(lb[0], lb[|entries|], entry);
+             && (forall i {:trigger VirtualSystemNextEntry(lb[i], lb[i+1], entries[i])} ::
+                 0 <= i < |entries| ==> VirtualSystemNextEntry(lb[i], lb[i+1], entries[i]))
+            ensures VirtualSystemNextEntry(lb[0], lb[|entries|], entry);
         {
             forall i | 0 <= i < |entries|
-                ensures SystemNextEntry(lb[i], lb[i+1], tree.children[i].entry);
+                ensures VirtualSystemNextEntry(lb[i], lb[i+1], tree.children[i].entry);
             {
                 assert entries[i] == tree.children[i].entry;
             }
@@ -207,4 +283,5 @@ module EventHandlerModule {
 
         assert TreeRootValid(tree);
     }
+*/
 }
