ironfleet/src/Dafny/Distributed/Concur/Movers.i.dfy
@@ -4,57 +4,57 @@ module MoversModule {
 
     import opened SystemModule
 
-    predicate ActionIsRightMover(action:Action)
+    predicate ActionIsRightMover(action:RealAction)
     {
-        action.ActionEvent? && (action.e.UdpReceiveEvent? || action.e.LockEvent?)
+        action.RealActionEvent? && (action.e.UdpReceiveEvent? || action.e.LockEvent?)
     }
 
-    predicate ActionIsLeftMover(action:Action)
+    predicate ActionIsLeftMover(action:RealAction)
     {
-        action.ActionEvent? && (action.e.UdpSendEvent? || action.e.UnlockEvent?)
+        action.RealActionEvent? && (action.e.UdpSendEvent? || action.e.UnlockEvent?)
     }
 
-    predicate EntryIsRightMover(entry:Entry)
+    predicate EntryIsRightMover(entry:RealEntry)
     {
         ActionIsRightMover(entry.action)
     }
 
-    predicate EntryIsLeftMover(entry:Entry)
+    predicate EntryIsLeftMover(entry:RealEntry)
     {
         ActionIsLeftMover(entry.action)
     }
 
     lemma lemma_MoverCommutativityForEntries(
-        entry1:Entry,
-        entry2:Entry,
-        ls1:SystemState,
-        ls2:SystemState,
-        ls3:SystemState
+        entry1:RealEntry,
+        entry2:RealEntry,
+        ls1:RealSystemState,
+        ls2:RealSystemState,
+        ls3:RealSystemState
         )
         returns
-        (ls2':SystemState)
+        (ls2':RealSystemState)
         requires entry1.actor != entry2.actor;
-        requires SystemNextEntry(ls1, ls2, entry1);
-        requires SystemNextEntry(ls2, ls3, entry2);
+        requires RealSystemNextEntry(ls1, ls2, entry1);
+        requires RealSystemNextEntry(ls2, ls3, entry2);
         requires EntryIsRightMover(entry1) || EntryIsLeftMover(entry2);
-        ensures  SystemNextEntry(ls1, ls2', entry2);
-        ensures  SystemNextEntry(ls2', ls3, entry1);
+        ensures  RealSystemNextEntry(ls1, ls2', entry2);
+        ensures  RealSystemNextEntry(ls2', ls3, entry1);
     {
-        if entry1.action.ActionEvent? && entry1.action.e.UdpReceiveEvent? {
+        if entry1.action.RealActionEvent? && entry1.action.e.UdpReceiveEvent? {
             ls2' := ls3;
         }
-        else if entry1.action.ActionEvent? && entry1.action.e.LockEvent? {
+        else if entry1.action.RealActionEvent? && entry1.action.e.LockEvent? {
             var lock := entry1.action.e.lock;
             ls2' := ls3.(locks := ls3.locks[lock := NoActor()]);
             assert ls2.locks[lock := NoActor()] == ls1.locks;
         }
-        else if entry2.action.ActionEvent? && entry2.action.e.UdpSendEvent? {
+        else if entry2.action.RealActionEvent? && entry2.action.e.UdpSendEvent? {
             ls2' := ls1.(sent_packets := ls1.sent_packets + {entry2.action.e.s});
-            if entry1.action.ActionEvent? && entry1.action.e.UdpSendEvent? {
+            if entry1.action.RealActionEvent? && entry1.action.e.UdpSendEvent? {
                 assert ls3.sent_packets == ls2'.sent_packets + {entry1.action.e.s};
             }
         }
-        else if entry2.action.ActionEvent? && entry2.action.e.UnlockEvent? {
+        else if entry2.action.RealActionEvent? && entry2.action.e.UnlockEvent? {
             var lock := entry2.action.e.unlock;
             ls2' := ls1.(locks := ls1.locks[lock := NoActor()]);
             assert ls2.locks[lock := NoActor()] == ls3.locks;
